Modulo challenges around endian-ness, naive version of AES-GCM goes through, assuming gf128_mul

src/crypto/aes/GHash_i.fst
@@ -68,3 +68,31 @@ let rec lemma_hash_append (h:quad32) (y_prev:quad32) (a b:ghash_plain) :
     assert(all_but_last ab == append a (all_but_last b));
   ()
    
+let lemma_hash_append3 (h y_init y_mid1 y_mid2 y_final:quad32) (s1 s2 s3:seq quad32) : Lemma
+  (requires y_init = Quad32 0 0 0 0 /\
+            y_mid1 = (if length s1 > 0 then ghash_incremental h y_init s1 else y_init) /\
+            y_mid2 = (if length s2 > 0 then ghash_incremental h y_mid1 s2 else y_mid1) /\
+            length s3 > 0 /\
+            y_final = ghash_incremental h y_mid2 s3)
+  (ensures y_final == ghash h (append s1 (append s2 s3)))
+  =
+  let s23 = append s2 s3 in
+  let s123 = append s1 s23 in
+  if length s1 = 0 then (
+    assert(eq s123 s23);
+    if length s2 = 0 then (
+      assert(eq s123 s3);
+      ghash_incremental_to_ghash h s3
+    ) else
+      lemma_hash_append h y_mid1 s2 s3;
+      ghash_incremental_to_ghash h s23
+  ) else if length s2 = 0 then (
+    assert(eq s123 (append s1 s3));
+    lemma_hash_append h y_init s1 s3;
+    ghash_incremental_to_ghash h (append s1 s3)
+  ) else (
+    lemma_hash_append h y_init s1 s23;
+    lemma_hash_append h y_mid1 s2 s3;
+    ghash_incremental_to_ghash h s123;
+    ()
+  )
