src/crypto/aes/GCM_s.fst
@@ -15,5 +15,5 @@ let gcm_encrypt (alg:algorithm) (key:aes_key alg) (iv:quad32) (p:gcm_plain) (a:g
   let c = gctr_encrypt (inc32 j0 1) p alg key in
   let hash_input = append a (append c (create 1 (Quad32 0 (length a) 0 (length c % nat32_max)))) in // Mod is needed, since F* can't see length c fits without a lemma
   let s = ghash h hash_input in
-  let t = gctr_encrypt j0 (create 1 s) in
+  let t = gctr_encrypt j0 (create 1 s) alg key in
   c, t
